SStructTT.lean
@@ -44,16 +44,16 @@ import SStructTT.SStruct.Dynamic.Preservation
 import SStructTT.SStruct.Dynamic.Progress
 import SStructTT.SStruct.Dynamic.Normalize
 
-import SStructTT.SStruct.Erasure.Syntax
-import SStructTT.SStruct.Erasure.Step
-import SStructTT.SStruct.Erasure.Erased
-import SStructTT.SStruct.Erasure.Renaming
-import SStructTT.SStruct.Erasure.Substitution
-import SStructTT.SStruct.Erasure.Inversion
-import SStructTT.SStruct.Erasure.Preservation
-import SStructTT.SStruct.Erasure.Progress
-import SStructTT.SStruct.Erasure.Normalize
+-- import SStructTT.SStruct.Erasure.Syntax
+-- import SStructTT.SStruct.Erasure.Step
+-- import SStructTT.SStruct.Erasure.Erased
+-- import SStructTT.SStruct.Erasure.Renaming
+-- import SStructTT.SStruct.Erasure.Substitution
+-- import SStructTT.SStruct.Erasure.Inversion
+-- import SStructTT.SStruct.Erasure.Preservation
+-- import SStructTT.SStruct.Erasure.Progress
+-- import SStructTT.SStruct.Erasure.Normalize
 
-import SStructTT.SStruct.Runtime.Heap
-import SStructTT.SStruct.Runtime.Resolution
-import SStructTT.SStruct.Runtime.Step
+-- import SStructTT.SStruct.Runtime.Heap
+-- import SStructTT.SStruct.Runtime.Resolution
+-- import SStructTT.SStruct.Runtime.Step
